erasure/theories/Extract.v
@@ -283,9 +283,9 @@ Inductive erases_deps (Σ : global_env) (Σ' : E.global_declarations) : E.term -
     erases_deps Σ Σ' discr ->
     Forall (fun br => erases_deps Σ Σ' br.2) brs ->
     erases_deps Σ Σ' (E.tCase p discr brs)
-| erases_deps_tProj p mdecl idecl mdecl' idecl' t :
-    declared_inductive Σ p.1.1 mdecl idecl ->
-    EGlobalEnv.declared_inductive Σ' p.1.1 mdecl' idecl' ->
+| erases_deps_tProj p mdecl idecl cdecl pdecl mdecl' idecl' cdecl' pdecl' t :
+    declared_projection Σ p mdecl idecl cdecl pdecl ->
+    EGlobalEnv.declared_projection Σ' p mdecl' idecl' cdecl' pdecl' ->
     erases_mutual_inductive_body mdecl mdecl' ->
     erases_one_inductive_body idecl idecl' ->
     erases_deps Σ Σ' t ->
